prove MapIAproof & clear minor codees

modules/HMod.v
@@ -1,20 +1,17 @@
 From CRIS.base_logic Require Import base_logic.
-Require Import Coqlib AList.
-Require Import sflib.
-Require Import ITreelib.
+
+Require Import Coqlib AList ITreelib.
 Require Import Any.
 Require Import Events.
 Require Import IRed.
 Require Import Behavior.
-Require Import PCM IPM.
+Require Import IPM.
 Require Import Skeleton Mod.
 Require Import PropExtensionality.
 Require Export HMod2Mod.
 
-Require Import PCM IPM. (* TODO : remove this when gra refactored *)
-
 Set Implicit Arguments.
-(* TODO : lift modules to ofes after asking about the well-formedness *)
+
 Definition fnsems_scopes {T} (fn : gname) (fnsems : alist gname (list string * T)) :=
   match (alist_find fn fnsems) with
   | Some (keys, body) => keys
@@ -22,26 +19,22 @@ Definition fnsems_scopes {T} (fn : gname) (fnsems : alist gname (list string * T
   end.
 
 Definition state_scopes (st : alist key Any.t) :=
-  (List.map (fst ∘ fst) st).
+  List.map (fst ∘ fst) st.
 
-Module HModSem.
-Section HMODSEM.
-  Context `{Σ : GRA.t}.
-  (* Notation hmodE := (hmodE (Σ:=Σ)) (only parsing). *)
-  
-  Set Printing Universes.
+Module HModSem. Section HModSem.
+  Context {Σ : GRA.t}.
 
   Record t : Type := mk {
     scopes : list string;
-    fnsems : alist gname (list string * (Any.t -> itree hmodE Any.t));
+    fnsems : alist gname (list string * (Any.t → itree hmodE Any.t));
     initial_st : alist key Any.t;
 
     well_scoped_fns :
-      forall fn, incl (fnsems_scopes fn fnsems) scopes;
+      ∀ fn, incl (fnsems_scopes fn fnsems) scopes;
     well_scoped_init :
       incl (state_scopes initial_st) scopes;
     nodup_fns :
-      List.NoDup scopes -> List.NoDup (List.map fst initial_st);
+      List.NoDup scopes → List.NoDup (List.map fst initial_st);
   }.
 
   Record wf (ms : t) : Prop := mk_wf {
@@ -50,7 +43,6 @@ Section HMODSEM.
   }.
 
   (**** Linking ****)
-
   Program Definition empty : t := {|
     scopes := [];
     fnsems := [];
@@ -108,41 +100,34 @@ Section HMODSEM.
   Qed.
 
   (**** Sandboxing ****)
-
   Definition handle_sandbox scopes : hmodE -< hmodE :=
-    (fun T e =>
-       match e with
-       | inr1 (inr1 (inr1 (inl1 (SPut (s,f) v)))) =>
+    λ T e,
+      match e with
+       | inr1 (inr1 (inr1 (inl1 (SPut (s, f) v)))) =>
            if existsb (String.eqb s) scopes then e else inr1 (inr1 (inr1 (inr1 (Choose T))))
-       | inr1 (inr1 (inr1 (inl1 (SGet (s,f))))) =>
+       | inr1 (inr1 (inr1 (inl1 (SGet (s, f))))) =>
            if existsb (String.eqb s) scopes then e else inr1 (inr1 (inr1 (inr1 (Choose T))))
        | _ => e
-       end).
+      end.
 
   Definition sandbox {T} scopes (itr : itree hmodE T) :=
     translate (handle_sandbox scopes) itr.
 
-  Definition sandbox_body (kb : list string * (Any.t -> itree hmodE Any.t)) :=
-    fun arg => sandbox kb.1 (kb.2 arg).
+  Definition sandbox_body (kb : list string * (Any.t → itree hmodE Any.t)) :=
+    λ arg, sandbox kb.1 (kb.2 arg).
 
   Definition to_mod (ms : t) (r : Σ) : ModSem.t := {|
     ModSem.fnsems := List.map (map_snd (interp_hp_fun ∘ sandbox_body)) ms.(fnsems);
     ModSem.initial_st := Any.pair (alist_encode ms.(initial_st)) r↑;
   |}.
-  (* Local Instance: Params to_mod 1 := {}.
-  Global Instance to_mod_proper ms :
-    Proper ((≡) ==> (⊣⊢)) (to_mod ms) := ne_proper _. *)
+End HModSem. End HModSem.
 
-End HMODSEM.
-End HModSem.
-
-Module HMod.
-Section HMOD.
+Module HMod. Section HMod.
   Context `{Σ : GRA.t}.
   Notation iProp := (iProp Σ).
 
   Record t : Type := mk {
-    modsem : Sk.t -> HModSem.t;
+    modsem : Sk.t → HModSem.t;
     sk : Sk.t;
   }.
 
@@ -159,19 +144,13 @@ Section HMOD.
   Definition addL (ms : list t) : t :=
     foldr add empty ms.
 
-  (* Definition to_mod (md : t) (r : Σ) : Mod.t := {| *)
-  (*   Mod.modsem := fun sk => HModSem.to_mod (md.(modsem) sk) r; *)
-  (*   Mod.sk := md.(sk); *)
-  (* |}. *)
+  Definition scopes (md : t) : Sk.t → list string :=
+    λ sk, (md.(modsem) sk).(HModSem.scopes).
 
-  Definition scopes (md : t) : Sk.t -> list string :=
-    fun sk => (md.(modsem) sk).(HModSem.scopes).
-
-  (* TODO : add a type of SK.t -> iProp and TC instances of equivalence *)
-  Definition modc : Type := (t * (Sk.t -> iProp))%type.
-  Local Instance modc_equiv : Equiv modc :=
-    (λ m1 m2, m1.1 = m2.1 ∧ ∀ sk, m1.2 sk ≡ m2.2 sk).
-  Local Instance modc_equiv_equiv : Equivalence modc_equiv.
+  (* TODO : add a type of SK.t → iProp and TC instances of equivalence *)
+  Definition modc : Type := (t * (Sk.t → iProp))%type.
+  Global Instance modc_equiv : Equiv modc := λ m1 m2, m1.1 = m2.1 ∧ ∀ sk, m1.2 sk ≡ m2.2 sk.
+  Global Instance modc_equiv_equiv : Equivalence modc_equiv.
   Proof.
     split; ss; ii.
     { inv H; split; clarify. i; rewrite H1; ss. }
@@ -183,14 +162,9 @@ Section HMOD.
 
   Definition empty_mc : modc := (empty, const(emp%I)).
 
-  Definition addc (C C' : Sk.t -> iProp) : Sk.t -> iProp :=
-    (fun sk => C sk ∗ C' sk)%I.
-
-  (* Definition add_mc (mc mc' : modc) : modc := *)
-  (*   (add mc.1 mc'.1, addc mc.2 mc'.2)%I. *)
-
-End HMOD.
-End HMod.
+  Definition addc (C C' : Sk.t → iProp) : Sk.t → iProp :=
+    (λ sk, C sk ∗ C' sk)%I.
+End HMod. End HMod.
 
 Infix "★" := HMod.add (at level 9, right associativity).
 Notation "◯" := HMod.empty (at level 9).
@@ -198,44 +172,32 @@ Infix "∗∗" := HMod.addc (at level 9, right associativity).
 
 Notation "░ it" := (HModSem.sandbox _ it) (at level 60, only printing).
 
-Section PROPERTIES.
-
+Section HModProperties.
   Context `{Σ : GRA.t}.
   Notation iProp := (iProp Σ).
 
   Lemma hmodsem_extensionality (ms1 ms2 : HModSem.t)
-    (SCOPE : HModSem.scopes ms1 = HModSem.scopes ms2)
-    (FNSEM : HModSem.fnsems ms1 = HModSem.fnsems ms2)
-    (INITS : HModSem.initial_st ms1 = HModSem.initial_st ms2)
-    (* (INITC : HModSem.initial_cond ms1 = HModSem.initial_cond ms2) *)
-    :
+      (SCOPE : HModSem.scopes ms1 = HModSem.scopes ms2)
+      (FNSEM : HModSem.fnsems ms1 = HModSem.fnsems ms2)
+      (INITS : HModSem.initial_st ms1 = HModSem.initial_st ms2) :
     ms1 = ms2.
-  Proof.
-    destruct ms1, ms2; ss. subst. f_equal; apply proof_irrelevance.
-  Qed.
+  Proof. destruct ms1, ms2; ss. subst. f_equal; apply proof_irrelevance. Qed.
 
-  Lemma hmodsem_add_assoc (ms1 ms2 ms3 : HModSem.t):
+  Lemma hmodsem_add_assoc (ms1 ms2 ms3 : HModSem.t) :
     HModSem.add (HModSem.add ms1 ms2) ms3 = HModSem.add ms1 (HModSem.add ms2 ms3).
   Proof.
     destruct ms1, ms2, ms3.
     apply hmodsem_extensionality; s; try rewrite app_assoc; eauto.
-    (* destruct initial_cond, initial_cond0, initial_cond1; ss. *)
-    (* rewrite iprop_sepconj_assoc. eauto. *)
   Qed.
 
-  Lemma hmodsem_add_empty_l ms:
+  Lemma hmodsem_add_empty_l (ms : HModSem.t) :
     HModSem.add HModSem.empty ms = ms.
-  Proof.
-    destruct ms. apply hmodsem_extensionality; s; eauto.
-  Qed.
+  Proof. destruct ms. apply hmodsem_extensionality; s; eauto. Qed.
 
-  Lemma hmodsem_add_empty_r ms:
-    HModSem.add ms HModSem.empty = ms.
-  Proof.
-    destruct ms. apply hmodsem_extensionality; s; try rewrite app_nil_r; eauto.
-  Qed.
+  Lemma hmodsem_add_empty_r ms : HModSem.add ms HModSem.empty = ms.
+  Proof. destruct ms. apply hmodsem_extensionality; s; try rewrite app_nil_r; eauto. Qed.
 
-  Lemma hmod_add_assoc (md1 md2 md3 : HMod.t):
+  Lemma hmod_add_assoc (md1 md2 md3 : HMod.t) :
     (md1 ★ md2) ★ md3 = md1 ★ md2 ★ md3.
   Proof.
     destruct md1, md2, md3. unfold HMod.add. s. f_equal.
@@ -243,132 +205,72 @@ Section PROPERTIES.
     - unfold Sk.add. rewrite app_assoc. eauto.
   Qed.
 
-  Lemma hmod_add_empty_l md:
-    ◯ ★ md = md.
+  Lemma hmod_add_empty_l (md : HMod.t) : ◯ ★ md = md.
   Proof.
-    destruct md. unfold HMod.add. s. f_equal.
-    extensionalities. apply hmodsem_add_empty_l.
+    destruct md. unfold HMod.add. s. f_equal. extensionalities. apply hmodsem_add_empty_l.
   Qed.
 
-  Lemma hmod_add_empty_r md:
-    md ★ ◯ = md.
+  Lemma hmod_add_empty_r (md : HMod.t) : md ★ ◯ = md.
   Proof.
     destruct md. unfold HMod.add. s. f_equal.
     - extensionalities. apply hmodsem_add_empty_r.
     - destruct sk; ss. unfold Sk.add. s. rewrite app_nil_r. eauto.
   Qed.
 
-  Lemma hmod_addL_app l l':
-    HMod.addL (l ++ l') = (HMod.addL l) ★ (HMod.addL l').
+  Lemma hmod_addL_app l l' : HMod.addL (l ++ l') = (HMod.addL l) ★ (HMod.addL l').
   Proof.
     induction l; s.
     - rewrite hmod_add_empty_l. eauto.
     - rewrite hmod_add_assoc. rewrite IHl. eauto.
   Qed.
 
-  (* Lemma iprop'_extensionality (P Q : iProp'):
-    iProp_pred P = iProp_pred Q -> P = Q.
+  Lemma hmod_addc_assoc (md : HMod.t) (P Q R : Sk.t → iProp) :
+    (md, (P ∗∗ Q) ∗∗ R) ≡ (md, P ∗∗ Q ∗∗ R).
   Proof.
-    i. destruct P, Q. ss. revert iProp_mono iProp_mono0.
-    rewrite H. i. f_equal. apply proof_irrelevance.
+    econs; ss.
+    intros sk; iSplit.
+    { iIntros "[[P Q] R]"; iFrame. }
+    { iIntros "[P [Q R]]"; iFrame. }
   Qed.
 
-  Lemma iprop_add_assoc (P Q R : iProp):
-    ((P ∗ Q) ∗ R)%I = (P ∗ (Q ∗ R))%I.
+  Lemma hmod_addc_empty_l (md : HMod.t) (P : Sk.t → iProp) :
+    (md, (const(emp%I)) ∗∗ P) ≡ (md, P).
   Proof.
-    unfold iProp, bi_car, bi_sep, Sepconj. unseal "iProp".
-    apply iprop'_extensionality. s.
-    extensionality r. apply propositional_extensionality.
-    split; i.
-    - des. subst. exists a0, (b0 ⋅ b). esplits; eauto.
-      rewrite URA.add_assoc. eauto.
-    - des. subst. exists (a ⋅ a0), b0. esplits; eauto.
-      rewrite URA.add_assoc. eauto.
+    econs; ss.
+    intros sk; iSplit.
+    { iIntros "[_ P]"; iFrame. }
+    { iIntros "P"; iFrame. rewrite /const //. }
   Qed.
 
-  Lemma iprop_add_empty_l (P : iProp):
-    (emp ∗ P)%I = P.
+  Lemma hmod_addc_empty_r (md : HMod.t) (P : Sk.t → iProp) :
+    (md, P ∗∗ (const(emp%I))) ≡ (md, P).
   Proof.
-    unfold iProp, bi_car, bi_sep, Sepconj, bi_emp, Emp. unseal "iProp".
-    apply iprop'_extensionality. s.
-    extensionality r. apply propositional_extensionality.
-    split; i.
-    - des. subst. eapply iProp_mono; eauto.
-      rr. esplits; eauto. rewrite URA.add_comm. eauto.
-    - exists ε, r. esplits; eauto.
-      rewrite URA.unit_idl. eauto.
+    econs; ss.
+    intros sk; iSplit.
+    { iIntros "[P _]"; iFrame. }
+    { iIntros "P"; iFrame. }
   Qed.
+End HModProperties.
 
-  Lemma iprop_add_empty_r (P : iProp):
-    (P ∗ emp)%I = P.
-  Proof.
-    unfold iProp, bi_car, bi_sep, Sepconj, bi_emp, Emp. unseal "iProp".
-    apply iprop'_extensionality. s.
-    extensionality r. apply propositional_extensionality.
-    split; i.
-    - des. subst. eapply iProp_mono; eauto.
-      rr. esplits; eauto.
-    - exists r, ε. esplits; eauto.
-      rewrite URA.add_comm. rewrite URA.unit_idl. eauto.
-  Qed. *)
-
-  (* Lemma hmod_addc_assoc (P Q R : Sk.t -> iProp) :
-    (P ∗∗ Q) ∗∗ R = P ∗∗ Q ∗∗ R.
-  Proof.
-    extensionalities. unfold HMod.addc.
-    (* Set Printing All. *)
-    rewrite /IPM.iProp /uPredI /bi_sep /uPred_sep.
-    Local Transparent upred.uPred_sep_aux. uPred_primitive.unseal.
-  Qed.
-
-  Lemma hmod_addc_empty_l (P : Sk.t -> iProp):
-    (const(emp%I)) ∗∗ P = P.
-  Proof.
-    extensionalities. unfold HMod.addc. rewrite iprop_add_empty_l. refl.
-  Qed.
-
-  Lemma hmod_addc_empty_r (P : Sk.t -> iProp):
-    P ∗∗ (const(emp%I)) = P.
-  Proof.
-    extensionalities. unfold HMod.addc. rewrite iprop_add_empty_r. refl.
-  Qed. *)
-
-End PROPERTIES.
-
-Module HModSB.
-Section RED.
+(* Sandboxing interpretation lemmas *)
+Module HModSB. Section HModSB.
   Context `{Σ : GRA.t}.
 
-  Lemma transl_bind
-    A B
-    scopes
-    (itr : itree hmodE A) (ktr : A -> itree hmodE B)
-    :
-    HModSem.sandbox scopes (itr >>= ktr) = a <- (HModSem.sandbox scopes itr);; (HModSem.sandbox scopes (ktr a))
-  .
+  Lemma transl_bind A B scopes (itr : itree hmodE A) (ktr : A → itree hmodE B) :
+    HModSem.sandbox scopes (itr >>= ktr)
+    = a <- (HModSem.sandbox scopes itr);; (HModSem.sandbox scopes (ktr a)).
   Proof. unfold HModSem.sandbox. rewrite (bisim_is_eq (translate_bind _ _ _)); eauto. Qed.
 
-  Lemma transl_tau
-    A
-    scopes
-    (itr : itree hmodE A)
-  :
-    HModSem.sandbox scopes (tau;; itr) = tau;; (HModSem.sandbox scopes itr)
-  .
+  Lemma transl_tau A scopes (itr : itree hmodE A) :
+    HModSem.sandbox scopes (tau;; itr) = tau;; (HModSem.sandbox scopes itr).
   Proof. unfold HModSem.sandbox. rewrite (bisim_is_eq (translate_tau _ _)); eauto. Qed.
 
-  Lemma transl_ret
-      A (a : A) scopes
-  :
-    HModSem.sandbox scopes (Ret a) = Ret a
-  .
+  Lemma transl_ret A (a : A) scopes :
+    HModSem.sandbox scopes (Ret a) = Ret a.
   Proof. unfold HModSem.sandbox. rewrite (bisim_is_eq (translate_ret _ _)); eauto. Qed.
 
-  Lemma transl_call {A} (e : callE A)
-    scopes
-  :
-  HModSem.sandbox scopes (trigger e) = trigger e
-  .
+  Lemma transl_call {A} (e : callE A) scopes :
+    HModSem.sandbox scopes (trigger e) = trigger e.
   Proof.
     unfold HModSem.sandbox, trigger.
     rewrite (bisim_is_eq (translate_vis _ _ _ _)). ss.
@@ -376,36 +278,25 @@ Section RED.
     rewrite (bisim_is_eq (translate_ret _ _)); eauto.
   Qed.
 
-  Lemma transl_put
-    scopes k v
-  :
-  HModSem.sandbox scopes (trigger (SPut k v)) =
-    if existsb (String.eqb k.1) scopes then trigger (SPut k v) else trigger (Choose _)
-  .
+  Lemma transl_put scopes k v :
+    HModSem.sandbox scopes (trigger (SPut k v))
+    = if existsb (String.eqb k.1) scopes then trigger (SPut k v) else trigger (Choose _).
   Proof.
     unfold HModSem.sandbox, trigger. destruct k. s.
     rewrite (bisim_is_eq (translate_vis _ _ _ _)). ss.
-    des_ifs; s; do 2 f_equal; extensionalities;
-      rewrite (bisim_is_eq (translate_ret _ _)); eauto.
+    des_ifs; s; do 2 f_equal; extensionalities; rewrite (bisim_is_eq (translate_ret _ _)); eauto.
   Qed.
 
-  Lemma transl_get
-    scopes k
-  :
-  HModSem.sandbox scopes (trigger (SGet k)) =
-    if existsb (String.eqb k.1) scopes then trigger (SGet k) else trigger (Choose Any.t)
-  .
+  Lemma transl_get scopes k :
+    HModSem.sandbox scopes (trigger (SGet k))
+    = if existsb (String.eqb k.1) scopes then trigger (SGet k) else trigger (Choose Any.t).
   Proof.
     unfold HModSem.sandbox, trigger. destruct k. s.
     rewrite (bisim_is_eq (translate_vis _ _ _ _)). ss.
-    des_ifs; s; do 2 f_equal; extensionalities;
-      rewrite (bisim_is_eq (translate_ret _ _)); eauto.
+    des_ifs; s; do 2 f_equal; extensionalities; rewrite (bisim_is_eq (translate_ret _ _)); eauto.
   Qed.
 
-  Lemma transl_core
-    T scopes
-    (e : coreE T)
-    :
+  Lemma transl_core T scopes (e : coreE T) :
     HModSem.sandbox scopes (trigger e) = trigger e.
   Proof.
     unfold HModSem.sandbox, trigger.
@@ -414,11 +305,8 @@ Section RED.
       rewrite (bisim_is_eq (translate_ret _ _)); eauto.
   Qed.
 
-  Lemma transl_ag {A} (e : agE A)
-    scopes
-  :
-    HModSem.sandbox scopes (trigger e) = trigger e
-  .
+  Lemma transl_ag {A} (e : agE A) scopes :
+    HModSem.sandbox scopes (trigger e) = trigger e.
   Proof.
     unfold HModSem.sandbox, trigger.
     rewrite (bisim_is_eq (translate_vis _ _ _ _)). ss.
@@ -426,11 +314,8 @@ Section RED.
     rewrite (bisim_is_eq (translate_ret _ _)); eauto.
   Qed.
 
-  Lemma transl_sch {A} (e : schE A)
-    scopes
-  :
-  HModSem.sandbox scopes (trigger e) = trigger e
-  .
+  Lemma transl_sch {A} (e : schE A) scopes :
+    HModSem.sandbox scopes (trigger e) = trigger e.
   Proof.
     unfold HModSem.sandbox, trigger.
     rewrite (bisim_is_eq (translate_vis _ _ _ _)). ss.
@@ -438,11 +323,8 @@ Section RED.
     rewrite (bisim_is_eq (translate_ret _ _)); eauto.
   Qed.
 
-  Lemma transl_unwrapU
-    R scopes (r : option R)
-  :
-    HModSem.sandbox scopes (unwrapU r) = unwrapU r
-  .
+  Lemma transl_unwrapU R scopes (r : option R) :
+    HModSem.sandbox scopes (unwrapU r) = unwrapU r.
   Proof.
     unfold unwrapU. destruct r.
     - apply transl_ret.
@@ -450,11 +332,8 @@ Section RED.
       f_equal. extensionalities. ss.
   Qed.
 
-  Lemma transl_unwrapN
-    R scopes (r : option R)
-  :
-    HModSem.sandbox scopes (unwrapN r) = unwrapN r
-  .
+  Lemma transl_unwrapN R scopes (r : option R) :
+    HModSem.sandbox scopes (unwrapN r) = unwrapN r.
   Proof.
     unfold unwrapN. destruct r.
     - apply transl_ret.
@@ -462,78 +341,13 @@ Section RED.
       f_equal. extensionalities. ss.
   Qed.
 
-  Lemma transl_asm
-    scopes P
-  :
-    HModSem.sandbox scopes (assume P) = assume P
-  .
+  Lemma transl_asm scopes P :
+    HModSem.sandbox scopes (assume P) = assume P.
   Proof.
     unfold assume. rewrite/__ transl_bind transl_core transl_ret. eauto.
   Qed.
 
-  Lemma transl_guar
-    scopes P
-  :
-    HModSem.sandbox scopes (guarantee P) = guarantee P
-  .
-  Proof.
-    unfold guarantee. rewrite/__ transl_bind transl_core transl_ret. eauto.
-  Qed.
-
-(*
-  Lemma transl_triggerUB
-    T scopes
-  :
-    HModSem.sandbox scopes (triggerUB : itree _ T) = triggerUB
-  .
-  Proof.
-    unfold triggerUB. rewrite transl_bind. f_equal.
-    { apply transl_coreE. }
-    extensionalities. ss.
-  Qed.
-
-  Lemma transl_triggerNB
-    T scopes
-  :
-    HModSem.sandbox scopes (triggerNB : itree _ T) = triggerNB
-  .
-  Proof.
-    unfold triggerNB. rewrite transl_bind. f_equal.
-    { apply transl_coreE. }
-    extensionalities. ss.
-  Qed.
-
-  Lemma transl_ext
-    T scopes (itr0 itr1 : itree _ T)
-    (EQ : itr0 = itr1)
-  :
-    HModSem.sandbox scopes itr0 = HModSem.sandbox scopes itr1
-  .
-  Proof. subst. refl. Qed.
- *)
-
-End RED.
-End HModSB.
-
-(* Section RDB. *)
-(*   Context `{Σ : GRA.t}. *)
-
-(*   Global Program Instance transl_rdb : red_database (mk_box (@translate)) := *)
-(*     mk_rdb *)
-(*     0 *)
-(*     (mk_box HModRed.transl_bind) *)
-(*     (mk_box HModRed.transl_tau) *)
-(*     (mk_box HModRed.transl_ret) *)
-(*     (mk_box HModRed.transl_putE) *)
-(*     (mk_box HModRed.transl_getE) *)
-(*     (mk_box HModRed.transl_callE) *)
-(*     (mk_box HModRed.transl_coreE) *)
-(*     (mk_box HModRed.transl_triggerUB) *)
-(*     (mk_box HModRed.transl_triggerNB) *)
-(*     (mk_box HModRed.transl_unwrapU) *)
-(*     (mk_box HModRed.transl_unwrapN) *)
-(*     (mk_box HModRed.transl_assume) *)
-(*     (mk_box HModRed.transl_guarantee) *)
-(*     (mk_box HModRed.transl_ext). *)
-
-(* End RDB. *)
+  Lemma transl_guar scopes P :
+    HModSem.sandbox scopes (guarantee P) = guarantee P.
+  Proof. rewrite /guarantee transl_bind transl_core transl_ret. eauto. Qed.
+End HModSB. End HModSB.
