examples/map/MapIAproof.v
@@ -1,30 +1,12 @@
-Require Import Coqlib ITreelib sflib.
-Require Import MapHeader MapASpec MapMSpec MapI MapM MapA ModSim MapIMproof MapMAproof MemA.
+Require Import Coqlib ITreelib.
+Require Import MapHeader MapASpec MapMSpec MapI ModSim MapIMproof MapMAproof MemA.
 Require Import ImpPrelude.
 Require Import Skeleton.
-Require Import PCM IPM.
-Require Import Events Behavior CtxRefine CtxRefineFacts.
-Require Import Relation_Definitions.
-
-(*** TODO : export these in Coqlib or Universe ***)
-Require Import Relation_Operators.
-Require Import RelationPairs.
-From ITree Require Import
-     Events.MapDefault.
-From ExtLib Require Import
-     Core.RelDec
-     Structures.Maps
-     Data.Map.FMapAList.
+Require Import IPM.
 
 Require Import STB.
-Require Import ISim SMod HMod Mod ModSimFacts.
-Require Import MainAdequacy CtxRefine.
-Require Import sProp sWorld World SRF.
-From stdpp Require Import coPset gmap namespaces.
-
-Set Implicit Arguments.
-
-Local Open Scope nat_scope.
+Require Import ISim SMod HMod.
+Require Import MainAdequacy CtxRefine CtxRefineFacts.
 
 Module MapIA. Section MapIA.
   Context `{!MapAS.G Σ, !MapMS.G Σ, !memG Σ}.
@@ -41,13 +23,11 @@ Module MapIA. Section MapIA.
       i. split; try refl. unfold MapMS.Stb. unseal "ccr". prove_nodup. }
     etrans; cycle 1.
     { eapply ctxr_frameR.
-      admit.
-      (* TODO : extend the definition of hmods *)
-      (* rewrite <-(hmod_addc_empty_l MapMS.InitCond). *)
-      (* eapply ctxr_cond_frameR. *)
-      (* eapply main_adequacy. eapply MapMA.sim; eauto. *)
-      (* i. split; try refl. unfold MapMS.Stb. unseal "ccr". prove_nodup. *)
+      rewrite -(hmod_addc_empty_l _ MapMS.InitCond).
+      eapply ctxr_cond_frameR, main_adequacy, MapMA.sim; eauto.
+      intros sk; split; try refl.
+      rewrite /MapMS.Stb; unseal "ccr"; prove_nodup.
     }
     refl.
-  Admitted.
+  Qed.
 End MapIA. End MapIA.
